\subsection{Mul233 }
See algorithm \ref{algo:Mul233}

\begin{lem}[Mul233] Let $(a_h,a_{\ell})$ a \textbf{double-double} number and $(b_h, b_m, b_{\ell})$ a   \textbf{triple-Double} number, $r_h$, $r_m$ and  $r_{\ell}$ result of $Mul233(a_h,a_{\ell},b_h,b_m,b_{\ell})$ for the $4$ modes of rounding, considering that there is no \textbf{overflow} so: $ \lvert r_{\ell} \rvert \le 4.u. \lvert r_m \rvert$ , $\lvert r_m \rvert \le u.(2.u + 2^{-\beta_o} +2^{-\beta_o -\beta_u}). \lvert r_h \rvert$ and $\lvert r_{\ell} \rvert \le u.(2.u + 2^{-\beta_o} +2^{-\beta_o -\beta_u}). \lvert r_h \rvert$.
\end{lem}

\begin{proof} \color{-yellow}
According to $Mul233$,we have:
\begin{itemize}
    \item $r_h + t_1 = Mul112(a_h,b_h)$ according to $Mul112$ $\Rightarrow$  $r_h + t_1 = a_h.b_h $ and  $\lvert t_1 \rvert \le u. \lvert r_h \rvert$ $\Rightarrow$
    $$\lvert a_h.b_h \rvert \le (1 + u). \lvert r_h \rvert $$
    $$\lvert a_h.b_h \rvert \le \frac{1}{u+1}. \lvert r_h \rvert $$
    \item $t_2 + t_3 = Mul112(a_h,b_m)$ according to $Mul112$ $\Rightarrow$ $t_2 + 
    t_3 = a_h.b_m$ and $\lvert t_3 \rvert \le u. \lvert t_2 \rvert$ $\Rightarrow$
    $$\lvert t_2 + t_3 \rvert \le \lvert a_h.b_m \rvert$$
    As $\lvert b_m \rvert \le 2^{-\beta_o}. \lvert b_h \rvert$ $\Rightarrow$ $\lvert a_h.b_m \rvert \le 2^{-\beta_o}. \lvert a_h.b_h \rvert$ $\Rightarrow$
    $$\lvert t_2 + t_3 \rvert \le 2^{-\beta_o}. \lvert a_h.b_h \rvert$$
    As $\lvert a_h.b_h \rvert \le \frac{1}{u+1}. \lvert r_h \rvert $
    $$\lvert t_2 + t_3 \rvert \le 2^{-\beta_o}. \frac{1}{u+1}. \lvert r_h \rvert$$
    As $\lvert t_3 \rvert \le u. \lvert t_2 \rvert$ $\Rightarrow$
    $$ (1-u). \lvert t_2 \rvert \le \lvert t_2 + t_3 \rvert $$
    $$ (1-u). \lvert t_2 \rvert \le 2^{-\beta_o}. \frac{1}{u+1}. \lvert r_h \rvert $$
     $$  \lvert t_2 \rvert \le 2^{-\beta_o}. \frac{1}{1-u^2}. \lvert r_h \rvert $$
     $\Rightarrow$
     $$  \lvert t_3 \rvert \le 2^{-\beta_o}. \frac{u}{1-u^2}. \lvert r_h \rvert $$
     So not to write the repetitive calculations, I give the results for $\lvert t_i \rvert $ with $4 \le i \le 9$:
     $$  \lvert t_4 \rvert \le 2^{-\beta_o -\beta_u}. \frac{1}{1-u^2}. \lvert r_h \rvert $$
     $$  \lvert t_5 \rvert \le 2^{-\beta_o -\beta_u}. \frac{u}{1-u^2}. \lvert r_h \rvert $$
      $$  \lvert t_6 \rvert \le \frac{u}{1-u^2}. \lvert r_h \rvert $$
      $$  \lvert t_7 \rvert \le \frac{u^2}{1-u^2}. \lvert r_h \rvert $$
      $$  \lvert t_8 \rvert \le 2^{-\beta_o}. \frac{u}{1-u^2}. \lvert r_h \rvert $$
      $$  \lvert t_9 \rvert \le 2^{-\beta_o}. \frac{u^2}{1-u^2}. \lvert r_h \rvert $$
    \item $t_{10} = \circ(a_{\ell}.b_{\ell})$ According to collary \ref{cor:ux}:  $t_{10} = a_{\ell}.b_{\ell}(1+\epsilon_5)$ with $\lvert \epsilon_5 \rvert \le u$ 
    but $\lvert a_{\ell} \rvert \le u. \lvert a_h \rvert$ and $\lvert b_{\ell} \rvert \le 2^{-\beta_o -\beta_u}. \lvert b_h \rvert$ $\Rightarrow$
    $$\lvert t_{10} \rvert \le u.2^{-\beta_o -\beta_u}.\lvert a_h.b_h \rvert.(1+u)$$
    $$\lvert t_{10} \rvert \le u.(1+u).2^{-\beta_o -\beta_u}.\frac{1}{u+1}. \lvert r_h \rvert$$
    $$\lvert t_{10} \rvert \le u.2^{-\beta_o -\beta_u}. \lvert r_h \rvert$$ 
    \item $t_{11} + t_{12} = Add222(t_2, t_3, t_4, t_5)$ according to $Add222$ $\Rightarrow$ $t_{11} + t_{12} = (t_2+ t_3 + t_4 + t_5).(1 + \epsilon_4)$ with $\lvert \epsilon_4 \rvert \le 6.u^2$ and $\lvert t_{12} \rvert \le 6.u.\lvert t_{11} \rvert$ $\Rightarrow$
    $$\lvert t_{11} + t_{12} \rvert \ge (1 - 6.u). \lvert t_{11} \rvert$$
    $\Rightarrow$
    $$(1 - 6.u). \lvert t_{11} \rvert \le (\lvert t_2 \rvert + \lvert t_3 \rvert + \lvert t_4 \rvert + \lvert t_5 \rvert).(1 + 6.u^2)$$
    $$\lvert t_{11} \rvert \le \frac{1 + 6.u^2}{1 - 6.u}(\lvert t_2 \rvert + \lvert t_3 \rvert + \lvert t_4 \rvert + \lvert t_5 \rvert)$$
    
    $$\lvert t_{11} \rvert \le \frac{1 + 6.u^2}{1 - 6.u}.(2^{-\beta_o}. \frac{1}{1-u^2}. \lvert r_h \rvert + 2^{-\beta_o}. \frac{u}{1-u^2}. \lvert r_h \rvert + 2^{-\beta_o -\beta_u}. \frac{1}{1-u^2}. \lvert r_h \rvert$$ 
    $$+ 2.2^{-\beta_o -\beta_u}. \frac{u}{1-u^2}. \lvert r_h \rvert)$$
    $$\lvert t_{11} \rvert \le \frac{(1 + 6.u^2).(u+1)}{(1 - 6.u).(1-u^2)}.(2^{-\beta_o} + 2^{-\beta_o -\beta_u}). \lvert r_h \rvert $$
    $$\lvert t_{12} \rvert \le \frac{(1 + 6.u^2).(u^2+u)}{(1 - 6.u).(1-u^2)}.(2^{-\beta_o} + 2^{-\beta_o -\beta_u}). \lvert r_h \rvert $$
    
    \item $t_{13} + t_{14} = Add222(t_6, t_7, t_8, t_9)$ according to $Add222$ 
    $\Rightarrow$ $t_{13} + t_{14} = (t_6+ t_7+ t_8 +t_9).(1 + \epsilon_3)$with 
    $\lvert \epsilon_3 \rvert \le 6.u^2$ and $\lvert t_{14} \rvert \le 6.u.\lvert t_{13} \rvert$ \\
    We do the same calculations as before.\\
    $\Rightarrow$ 
    $$\lvert t_{13} \rvert \le \frac{1}{1-6.u}.(\lvert t_6 \rvert + \lvert t_7 \rvert + \lvert t_8 \rvert + \lvert t_9 \rvert).(1 + 6.u^2)$$
    $$\lvert t_{13} \rvert \le \frac{1 + 6.u^2}{1-6.u}.(\frac{u}{1-u^2}. \lvert r_h \rvert + \frac{u^2}{1-u^2}. \lvert r_h \rvert + 2^{-\beta_o}. \frac{u}{1-u^2}. \lvert r_h \rvert + 2^{-\beta_o}. \frac{u^2}{1-u^2}. \lvert r_h \rvert).$$
    $$\lvert t_{13} \rvert \le \frac{(1 + 6.u^2).(u^2+u).(u+1)^2}{(1-6.u).(1-u^2)}.(1 +  2^{-\beta_o}) .\lvert r_h \rvert.$$
    $$\lvert t_{14} \rvert \le \frac{(1 + 6.u^2).(u^3+u^2).(u+1)^2}{(1-6.u).(1-u^2)}.(1 +  2^{-\beta_o}) .\lvert r_h \rvert.$$
    we do the same calculation for $t_{15}$ and $t_{16}$, after the calculations then the simplifications, we have:
    $$\lvert t_{15} \rvert \le \frac{(1+6.u^2).(u+1)^2}{(1-6.u).(1-u^2)}.(u.(u+1)^2 + (u^3+2.u^2+u+1).2^{-\beta_o} +2^{-\beta_o -\beta_u}). \lvert r_h \rvert$$
    $$\lvert t_{16} \rvert \le \frac{u.(1+6.u^2).(u+1)^2}{(1-6.u).(1-u^2)}.(u.(u+1)^2 + (u^3+2.u^2+u+1).2^{-\beta_o} +2^{-\beta_o -\beta_u}). \lvert r_h \rvert$$
    \item $t_{17} +t_{18} = Add112(t_1,t_{10})$ according to $Add112$ $\Rightarrow$
    $t_{17} +t_{18} = t_1+t_{10}$ and $\lvert t_{18} \rvert \le u.\lvert t_{17} \rvert$, as done before  $\Rightarrow$
    $$\lvert t_{17} \rvert \le \lvert \frac{1}{1-u} \rvert .(\lvert t_1 \rvert + \lvert t_{10} \rvert)$$
    $$\lvert t_{17} \rvert \le \lvert \frac{1}{1-u} \rvert .(u. \lvert r_h \rvert + u.2^{-\beta_o -\beta_u}. \lvert r_h \rvert)$$
    $$\lvert t_{17} \rvert \le \lvert \frac{u}{1-u} \rvert .(\lvert r_h \rvert + 2^{-\beta_o -\beta_u}. \lvert r_h \rvert)$$
   $$\lvert t_{18} \rvert \le \lvert \frac{u^2}{1-u} \rvert .(\lvert r_h \rvert + 2^{-\beta_o -\beta_u}. \lvert r_h \rvert)$$
    \item $r_m+r_{\ell} = Add222(t_{17},t_{18},t_{15},t_{16})$ according to $Add222$ $\Rightarrow$ $r_m+r_{\ell} = (t_{17}+t_{18}+t_{15}+t_{16})(1+\epsilon_1)$ with $\lvert \epsilon_1 \rvert \le 6.u^2$ and $\lvert r_{\ell} \rvert \le 6.u.\lvert r_m \rvert $, after calculation :
    $$\lvert r_m \rvert \le \frac{1}{1-6.u}.(\lvert t_{17} \rvert + \lvert t_{18} \rvert + \lvert t_{15} \rvert + \lvert t_{16} \rvert).(1 + 6.u^2)$$
    after we calculate:
    $$\lvert r_m \rvert \le (2.u + 2^{-\beta_o} +2^{-\beta_o -\beta_u}). \lvert r_h \rvert$$
    
    and 
    $$\lvert r_{\ell} \rvert \le u.(2.u + 2^{-\beta_o} +2^{-\beta_o -\beta_u}). \lvert r_h \rvert$$
\end{itemize}
\end{proof}

\begin{theo}[Relative error algorithm $Mul233$]
Let $(a_h,a_{\ell})$ a \textbf{double-double} number and $(b_h,b_m,b_{\ell})$ a \textbf{triple-double} number are the arguments of the function $Mul233$.\\
So:\\
$$r_h +r_m +r_{\ell} = (a_h + a_{\ell}). (b_h+ b_m +b_{\ell})).(1+\epsilon)$$ with $\lvert \epsilon \rvert \le \frac{24.u^3  + 19.u^2.2^{-\beta_o} + 20.u^2.2^{-\beta_o -\beta_u}}{1 - (u + (1+ u).2^{-\beta_o} + (1+u).2^{-\beta_o -\beta_u})} \le  48.u^3  + 19.u^2.2^{-\beta_o+1} + 5.u^2.2^{-\beta_o -\beta_u+3}$
\end{theo}
\begin{proof}[10pt] \color{-yellow}
According to  the conditions of $Mul233$, we begin to calculate $r_m + r_{\ell}$:\\
$r_m + r_{\ell} = Add222(t_{17},t_{18},t_{15},t_{16})$ According to $Add222$ $\Rightarrow$ $r_m + r_{\ell} = (t_{17}+t_{18}+t_{15}+t_{16}).(1+\epsilon_1)$ with $\lvert \epsilon_1 \rvert \le 6.u^2$
As $t_{17}+t_{18} = t_1 + t_{10}$ and $t_{15}+t_{16} = 
(t_{11}+t_{12}+t_{13}+t_{14}).(1+\epsilon_2)$ with $\lvert \epsilon_2 \rvert \le 6.u^2$
$$r_m + r_{\ell} = (t_1 + 
t_{10}+(t_{11}+t_{12}+t_{13}+t_{14}).(1+\epsilon_2)).(1+\epsilon_1) $$
As $t_{13}+t_{14} = (t_6+t_7+t_8+t_9)(1+\epsilon_3)$ and $t_{11}+t_{12} = 
(t_2+t_3+t_4+t_5)(1+\epsilon_4)$ with $\lvert \epsilon_2 \rvert \le 6.u^2$ and $\lvert 
\epsilon_3 \rvert \le 6.u^2$ $\Rightarrow$
$$r_m + r_{\ell} = (t_1 + 
t_{10}+((t_2+t_3+t_4+t_5)(1+\epsilon_4)+(t_6+t_7+t_8+t_9)(1+\epsilon_3)).(1+\epsilon_2))
.(1+\epsilon_1) $$
As $t_2+t_3 = a_h.b_m$, $t_4 + t_5 = a_h.b_{\ell}$, $t_6+t_7 = a_{\ell}.b_h$ and $t_8 + 
t_9 = a_{\ell}.b_m$ $\Rightarrow$
$$r_m + r_{\ell} = (t_1 + 
t_{10}+((a_h.b_m+a_h.b_{\ell})(1+\epsilon_4)+(a_{\ell}.b_h+a_{\ell}.b_m)(1+\epsilon_3)).(1+\epsilon_2))
.(1+\epsilon_1) $$
As $t_{10} = a_{\ell}.b_{\ell}.(1+\epsilon_5)$ with $\lvert \epsilon_5 \rvert \le u$ 
$\Rightarrow$
$$r_m + r_{\ell} = (t_1 + 
a_{\ell}.b_{\ell}.(1+\epsilon_5)+((a_h.b_m+a_h.b_{\ell})(1+\epsilon_4)+(a_{\ell}.b_h+a_{\ell}.b_m)(1+\epsilon_3)).(1+\epsilon_2))
.(1+\epsilon_1) $$
As $r_h +t_1 = a_h.b_h$ $\Rightarrow$
$$r_h + r_m + r_{\ell} = (a_h + a_{\ell}).(b_h + b_m + b_{\ell})+\delta $$
with $\delta = t_1.\epsilon_1 +  a_{\ell}.b_{\ell}.(\epsilon_1 + \epsilon_5 + \epsilon_1.\epsilon_5) + (a_h.b_m + a_h.b_{\ell}).(\epsilon_1 +\epsilon_2 \epsilon_4 + \epsilon_1.\epsilon_2 + \epsilon_1.\epsilon_4 + \epsilon_2.\epsilon_4 + \epsilon_1.\epsilon_2.\epsilon_4)
+ (a_{\ell}.b_h + a_{\ell}.b_m).(\epsilon_1 +\epsilon_3 \epsilon_4 + \epsilon_1.\epsilon_3 + \epsilon_1.\epsilon_4 + \epsilon_3.\epsilon_4 + \epsilon_1.\epsilon_3.\epsilon_4)$.\\
We seek the upper bound of $\lvert \delta \rvert$ in function of $\lvert a_h.b_h \rvert$:
$$\lvert \delta \rvert \le \lvert t_1.\epsilon_1 \rvert +  \lvert a_{\ell}.b_{\ell}.(\epsilon_1 + \epsilon_5 + \epsilon_1.\epsilon_5) \rvert  + ( \lvert a_h.b_m \rvert + \lvert a_h.b_{\ell} \rvert).\lvert \epsilon_1 +\epsilon_2 \epsilon_4 + \epsilon_1.\epsilon_2 + \epsilon_1.\epsilon_4 + \epsilon_2.\epsilon_4 + \epsilon_1.\epsilon_2.\epsilon_4 \rvert $$
$$+ (\lvert a_{\ell}.b_h \rvert + \lvert a_{\ell}.b_m \rvert). \lvert \epsilon_1 +\epsilon_3 \epsilon_4 + \epsilon_1.\epsilon_3 + \epsilon_1.\epsilon_4 + \epsilon_3.\epsilon_4 + \epsilon_1.\epsilon_3.\epsilon_4 \rvert$$
$$\lvert \delta \rvert \le 6.u^2.\lvert t_1 \rvert +  (6.u^3 +6.u^2 +u).\lvert a_{\ell}.b_{\ell}. \rvert  + (216.u^6+108.u^4 + 18.u^2).( \lvert a_h.b_m \rvert + \lvert a_h.b_{\ell} \rvert + \lvert a_{\ell}.b_h \rvert + \lvert a_{\ell}.b_m \rvert) $$
We seek the upper bound of $ \lvert a_h.b_m \rvert$, $\lvert a_h.b_{\ell} \rvert$, $\lvert a_{\ell}.b_h \rvert$, $\lvert a_{\ell}.b_m \rvert$ and $\lvert a_{\ell}.b_{\ell} \rvert $ in function of $\lvert a_h.b_h \rvert $.\\
We have:
$$ \lvert a_h.b_m \rvert \le 2^{-\beta_o}.\lvert a_h.b_h \rvert$$
$$ \lvert a_h.b_{\ell} \rvert \le 2^{-\beta_o -\beta_u}.\lvert a_h.b_h \rvert$$
$$ \lvert a_{\ell}.b_h \rvert \le u.\lvert a_h.b_h \rvert$$
$$ \lvert a_{\ell}.b_m \rvert \le u.2^{-\beta_o}.\lvert a_h.b_h \rvert$$
$$ \lvert a_{\ell}.b_{\ell} \rvert \le u.2^{-\beta_o -\beta_u}.\lvert a_h.b_h \rvert$$
We search the upper bound of  $(\lvert a_h.b_m \rvert + \lvert a_h.b_{\ell} \rvert + \lvert a_{\ell}.b_h \rvert + \lvert a_{\ell}.b_m \rvert )$ in function of $\lvert a_h.b_h \rvert$
$$\lvert a_h.b_m \rvert + \lvert a_h.b_{\ell} \rvert + \lvert a_{\ell}.b_h \rvert + \lvert a_{\ell}.b_m \rvert \le 2^{-\beta_o}.\lvert a_h.b_h \rvert + 2^{-\beta_o -\beta_u}.\lvert a_h.b_h \rvert + u.\lvert a_h.b_h \rvert + u.2^{-\beta_o}.\lvert a_h.b_h \rvert $$
$$\lvert a_h.b_m \rvert + \lvert a_h.b_{\ell} \rvert + \lvert a_{\ell}.b_h \rvert + \lvert a_{\ell}.b_m \rvert \le (u + (1+ u).2^{-\beta_o} + 2^{-\beta_o -\beta_u}).\lvert a_h.b_h \rvert $$
as $\lvert a_{\ell}.b_{\ell} \rvert \le u.2^{-\beta_o -\beta_u}.\lvert a_h.b_h \rvert$ \\
According to $Mul112$, we have :
$$\lvert t_1 \rvert \le u. \lvert r_h \rvert \ and \ r_h + t_1 = a_h.b_h$$
We begin to calculate the lower bound of $\lvert r_h + t_1 \rvert $ compared to $\lvert r_h \rvert$.\\
As $\lvert t_1 \rvert \le u. \lvert r_h \rvert$, we have :
$$\lvert r_h + t_1 \rvert \ge (1 - u). \lvert r_h \rvert$$
$\Rightarrow$
$$(1 - u). \lvert r_h \rvert \le \lvert a_h.b_h \rvert$$
$$ \lvert r_h \rvert \le \frac{1}{1-u}.\lvert a_h.b_h \rvert$$
$\Rightarrow$
$$ \lvert t_1 \rvert \le \frac{u}{1-u}.\lvert a_h.b_h \rvert$$
$$\lvert \delta \rvert \le (\frac{6u^3}{1-u}. +  (6.u^3 +6.u^2 +u).u.2^{-\beta_o -\beta_u}  + (216.u^6+108.u^4 + 18.u^2).(u + (1+ u).2^{-\beta_o} + 2^{-\beta_o -\beta_u})).\lvert a_h.b_h \rvert $$
we simplify with the upper bounds of each coefficient.
$$\lvert \delta \rvert \le (24.u^3  + 19.u^2.2^{-\beta_o} + 20.u^2.2^{-\beta_o -\beta_u}).\lvert a_h.b_h \rvert $$
Now, we seek the lower bound of $\lvert a_h.b_h \rvert $ in function of $\lvert (a_h +a_{\ell}).(b_h + b_m +b_{\ell}) \rvert$, as $\lvert a_h.b_m \rvert + \lvert a_h.b_{\ell} \rvert + \lvert a_{\ell}.b_h \rvert + \lvert a_{\ell}.b_m \rvert \le (u + (1+ u).2^{-\beta_o} + 2^{-\beta_o -\beta_u}).\lvert a_h.b_h \rvert $ and $\lvert a_{\ell}.b_{\ell} \rvert \le u.2^{-\beta_o -\beta_u}.\lvert a_h.b_h \rvert$ $\Rightarrow$
$$\lvert a_h.b_m+a_h.b_{\ell}+a_{\ell}.b_h+a_{\ell}.b_m + a_{\ell}.b_{\ell}\rvert \le \lvert a_h.b_m \rvert + \lvert a_h.b_{\ell} \rvert + \lvert a_{\ell}.b_h \rvert + \lvert a_{\ell}.b_m \rvert + \lvert a_{\ell}.b_{\ell} \rvert $$
$$\lvert a_h.b_m+a_h.b_{\ell}+a_{\ell}.b_h+a_{\ell}.b_m + a_{\ell}.b_{\ell}\rvert \le 
(u + (1+ u).2^{-\beta_o} + (1+u).2^{-\beta_o -\beta_u}).\lvert a_h.b_h \rvert$$
So we have:
$$\lvert (a_h +a_{\ell}).(b_h + b_m +b_{\ell}) \rvert \ge (1 - (u + (1+ u).2^{-\beta_o} + (1+u).2^{-\beta_o -\beta_u})).\lvert a_h.b_h \rvert$$
$$\lvert a_h.b_h \rvert \le \frac{1}{1 - (u + (1+ u).2^{-\beta_o} + (1+u).2^{-\beta_o -\beta_u})}.\lvert (a_h +a_{\ell}).(b_h + b_m +b_{\ell}) \rvert$$
at the end:
$$\lvert \delta \rvert \le \frac{24.u^3  + 19.u^2.2^{-\beta_o} + 20.u^2.2^{-\beta_o -\beta_u}}{1 - (u + (1+ u).2^{-\beta_o} + (1+u).2^{-\beta_o -\beta_u})}.\lvert (a_h +a_{\ell}).(b_h + b_m +b_{\ell}) \rvert $$
$\Rightarrow$
$\lvert \epsilon \rvert \le \frac{24.u^3  + 19.u^2.2^{-\beta_o} + 20.u^2.2^{-\beta_o -\beta_u}}{1 - (u + (1+ u).2^{-\beta_o} + (1+u).2^{-\beta_o -\beta_u})} $\\
\ \\
As $\beta_o \ge 2$ and $\beta_u \ge 1$ $\Rightarrow$ $1 - (u + (1+ u).2^{-\beta_o} + (1+u).2^{-\beta_o -\beta_u}) \ge \frac{1}{2}$ $\Rightarrow$\\
$\lvert \epsilon \rvert \le 48.u^3  + 19.u^2.2^{-\beta_o+1} + 5.u^2.2^{-\beta_o -\beta_u+3} $
\end{proof}